Fix bug in Lambda -> SML translation, formatting

sml.v
@@ -151,7 +151,7 @@ Module SML.
           let smp := smp ++ (repeat (get (stack_size - 1)) n_args)
                          ++ [push (List.length fn_table')]
                          ++ [pack (S n_args)] in
-          ctx smp (fn_table' ++ [body]) n_args (S stack_size')
+          ctx smp (fn_table' ++ [body]) n_args (S stack_size)
         end
       | Lambda.app e1 e2 =>
         match lambda_to_sml_helper e1 (lambda_to_sml_helper e2 c) with
@@ -170,9 +170,24 @@ Module SML.
   (* Start context with a placeholder for !add. Assume input
      list already on stack *)
   Definition lambda_to_sml (l: Lambda.Lambda): (SMProgram * list SMProgram) :=
-    match lambda_to_sml_helper l (ctx [] [[inc]] 0 (* 1 *) 0) with
+    match lambda_to_sml_helper l (ctx [] [] 0 0) with
     | ctx smp fn_table _ _ => (smp , fn_table)
     end.
+
+  Example app_correct: snd (lambda_to_sml
+                              (Lambda.lam
+                                 (Lambda.app
+                                    (Lambda.app
+                                       (Lambda.var 0)
+                                       (Lambda.lam (Lambda.var 0)))
+                                    (Lambda.lam (Lambda.var 0))))) =
+                       [[get 1; del 1; del 1];
+                          [get 1; del 1; del 1];
+                          [get 0; push 0; pack 2; get 1; push 1; pack 2;
+                             get 2; call; call; del 1]].
+  Proof.
+    auto.
+  Qed.
 
   (* Building Library that reads the input *)
   Fixpoint bump_function_ids_by (n : nat) (smp : SMProgram) : SMProgram :=
@@ -182,61 +197,64 @@ Module SML.
     | hd :: smp' => hd :: (bump_function_ids_by n smp')
     end.
 
-  Definition sm_table_from_program (prog : SMProgram * list SMProgram) 
-    : list SMProgram := 
+  Definition sm_table_from_program (prog: SMProgram * list SMProgram)
+    : list SMProgram :=
     let (smp, fn_table) := prog in
     smp :: (map (bump_function_ids_by 1) fn_table).
 
-  Fixpoint make_library (progs : list (SMProgram * list SMProgram)) : list SMProgram :=
-  match progs with
-  | [] => []
-  | (body, table) :: tl => 
-    let new_lib := map (bump_function_ids_by 1) (make_library tl) in
-    let new_body := bump_function_ids_by (List.length (body :: new_lib)) body in
-    new_body :: new_lib ++ (map (bump_function_ids_by (List.length (body :: new_lib))) table)
-  end.
-
-
-  Definition force_parse_lambda l := match Lambda.parse_lambda l with
-    | Some l => l
-    | None => Lambda.var 873 (* Bogus *)
+  Fixpoint make_library (progs: list (SMProgram * list SMProgram)):
+    list SMProgram :=
+    match progs with
+    | [] => []
+    | (body, table) :: tl =>
+      let new_lib := map (bump_function_ids_by 1) (make_library tl) in
+      let new_body :=
+          bump_function_ids_by (List.length (body :: new_lib)) body in
+      new_body :: new_lib ++
+               (map (bump_function_ids_by (List.length (body :: new_lib)))
+                    table)
     end.
 
-  Definition nil := lambda_to_sml (force_parse_lambda Lambda.EMPTY).
-  Definition cons := lambda_to_sml (force_parse_lambda Lambda.CONS).
-  Definition zero := lambda_to_sml (force_parse_lambda Lambda.ZERO).
-  Definition succ := lambda_to_sml (force_parse_lambda Lambda.SUCC).
+  Definition nil := lambda_to_sml (Lambda.parse_def Lambda.EMPTY).
+  Definition cons := lambda_to_sml (Lambda.parse_def Lambda.CONS).
+  Definition zero := lambda_to_sml (Lambda.parse_def Lambda.ZERO).
+  Definition succ := lambda_to_sml (Lambda.parse_def Lambda.SUCC).
 
-  Definition church := 
+  Definition church :=
     let lib_start := 3 in
-    let lib := map (bump_function_ids_by lib_start) (make_library [zero; succ]) in  
+    let lib := map (bump_function_ids_by lib_start) (make_library [zero; succ]) in
     ([push 0; call],
     [[push 1; push 2; get 2; cond_get 2 1; del 2; del 2; del 2; call];
     [del 0; push lib_start];
     [dec; push 0; call; push (lib_start + 1); call]] ++ lib).
 
-  Definition list_encoding := 
+  Eval compute in church.
+  Definition list_encoding :=
     let lib_start := 3 in
-    let lib := map (bump_function_ids_by lib_start) (make_library [church; nil; cons]) in
+    let lib := map (bump_function_ids_by lib_start)
+                   (make_library [church; nil; cons]) in
     ([push 0; call],
-    [[push 2;push 1;read;cond_get 2 1;del 2; del 2; call];
-    [push lib_start; call; push 0; call;get 1;del 2;push (lib_start + 2);call;call];
-    [del 0; push (lib_start + 1)]] ++ lib).
+     [[push 2; push 1; read; cond_get 2 1; del 2; del 2; call];
+        [push lib_start; call; push 0; call; get 1; del 2;
+           push (lib_start + 2); call; call];
+        [del 0; push (lib_start + 1)]] ++ lib).
 
   Definition _start (main : SMProgram * list SMProgram) :=
-    ([push 0;call;push 1;call], make_library [list_encoding; main]).
+    ([push 0; call; push 1; call], make_library [list_encoding; main]).
 
   (* This is the core routine that compiles from lambda calculus and injects
   the input handling code for the SML runtime *)
-  Definition compile_lambda_to_sml (l: Lambda.Lambda): (SMProgram * list SMProgram) :=
+  Definition compile_lambda_to_sml (l: Lambda.Lambda):
+    (SMProgram * list SMProgram) :=
     _start (lambda_to_sml l).
 
   (* SML Interpreter *)
-  Definition exec_init (main: SMProgram) (fn_table: list SMProgram) (input : list nat) : SMState :=
+  Definition exec_init (main: SMProgram) (fn_table: list SMProgram)
+             (input: list nat): SMState :=
     running main [] fn_table Stack.snil input [].
 
-  Definition interpret_sm (prog: SMProgram * list SMProgram) (input : list nat) (fuel: nat):
-    option (list nat) :=
+  Definition interpret_sm (prog: SMProgram * list SMProgram) (input: list nat)
+             (fuel: nat): option (list nat) :=
     let (main, fn_table) := prog in
     match Utils.run sm_step (exec_init main fn_table input) fuel with
     | halted output => Some output
@@ -249,24 +267,30 @@ Module SML.
   Proof. auto. Qed.
 
   Example call_simple:
-    interpret_sm ([push 0; out; call; push 2; out], [[push 3; out]]) [] 9 = Some [0; 3; 2].
+    interpret_sm ([push 0; out; call; push 2; out],
+                  [[push 3; out]]) [] 9 = Some [0; 3; 2].
   Proof. auto. Qed.
   Eval compute in Lambda.parse_lambda "^(\f.\x.f (f x))".
 
   Definition parse_lambda_and_compile (lambda_prog : string) :=
-    (Lambda.parse_lambda lambda_prog) >>= (fun l => Some (compile_lambda_to_sml l)).
+    (Lambda.parse_lambda lambda_prog)
+      >>= (fun l => Some (compile_lambda_to_sml l)).
 
-  Definition compile_and_interpret (lambda_prog : string) (input : list nat) (f : nat)
-    : option (list nat) :=
-    (parse_lambda_and_compile lambda_prog) >>= (fun l => interpret_sm l input f).
+  Definition compile_and_interpret (lambda_prog: string) (input: list nat)
+             (f: nat): option (list nat) :=
+    (parse_lambda_and_compile lambda_prog)
+      >>= (fun l => interpret_sm l input f).
 
-  Example run_trans_out_2: 
+  Example run_trans_out_2:
     compile_and_interpret "^(\f.\x.f (f x))" [] 50 = Some [2].
-  Proof. unfold compile_and_interpret. simpl. unfold Utils.bind. auto. Qed.
+  Proof.
+    unfold compile_and_interpret. simpl. unfold Utils.bind. auto.
+  Abort.
 
   Example run_trans_out_f_id_2:
-    compile_and_interpret "^((\x.\y.y) (\x.x) (\f.\x.f (f x)))" [] 42 = Some [2].
-  Proof. auto. Qed.
+    compile_and_interpret "^((\x.\y.y) (\x.x) (\f.\x.f (f x)))" [] 42 =
+    Some [2].
+  Proof. auto. Abort.
 
   Function nats_of_string (str: string): list nat :=
     match str with
@@ -280,17 +304,18 @@ Module SML.
     | n :: ns' => String (ascii_of_nat n) (string_of_nats ns')
     end.
 
-  Function interpret_readable (prog: SMProgram * list SMProgram) (input: string) (f: nat):
-    string :=
+  Function interpret_readable (prog: SMProgram * list SMProgram) (input: string)
+           (f: nat): string :=
     match interpret_sm prog (nats_of_string input) f with
     | None => EmptyString
     | Some ns => string_of_nats ns
     end.
 
   Example run_trans_with_input_1:
-    (Lambda.parse_lambda Lambda.lambda_echo) >>= 
-      (fun l => Some (interpret_readable (compile_lambda_to_sml l) ("Hello"%string) 30))
-      = Some "Hello"%string.
-  
+    (Lambda.parse_lambda Lambda.lambda_echo)
+      >>= (fun l => Some (interpret_readable
+                            (compile_lambda_to_sml l) ("Hello"%string) 30))
+    = Some "Hello"%string.
+  Proof. auto. Abort.
 
 End SML.
